\documentclass{article}
\usepackage[utf8]{inputenc}
\usepackage{amsmath}
\usepackage{graphicx}
\usepackage{physics}
\usepackage{listings}
\begin{document}
\section{Problem 3}
\subsection{Definitions}
a few definitions will be made:
\begin{align*}
    x &\equiv x_i\\
    x+h &\equiv x_{i+1}\\
    u(x_i) &\equiv u_i\\
    f(x_i) &\equiv f_i\\
\end{align*}
\subsection{Taylor series}
The taylor expansion is defined for a function $u(x)$ around the region $x=a$:
\begin{align*}
    u(x) = \sum_{n=0}^{\infty} \frac{u^{(n)}(a)}{n!}(x-a)^n
\end{align*}
alternatively it can be expressed
\begin{align}
    \label{eq:idk_yet}
    u(x) = u(a) + u'(a)(x+a) + O(h)
\end{align}
Where $O(h)$ is the error function.
for $a=x-h$, \ref{eq:idk_yet} becomes
\begin{align*}
    &u(x) = u(x-h) + u'(x-h)(x - (x-h)) + O(h)\\
    &= u(x-h) + u'(x-h)h + O(h)\\
    &\Rightarrow u_i =  u_{i-1}'h +u_{i-1} + O(h)\\
    &\Rightarrow  u_{i-1}' = \frac{u_i - u_{i-1}}{h} + O(h)\\
    &\Rightarrow u_i=  \frac{u_{i+1} - u_{i}}{h} + O(h)\\
\end{align*}
Alternatively for $a = x+h$
\begin{align*}
    &u(x) = u(x+h) - u'(x+h)h + O(h)\\
    &\Rightarrow u_i = u_{i+1} - u_{i+1}'h + O(h)\\
    &\Rightarrow u_{i+1}' =\frac{u_{i+1} - u_{i}}{h}\\
    &\Rightarrow u_{i}' =\frac{u_{i} - u_{i-1}}{h}\\
\end{align*}
\subsection{Solving for second derivative of u}
\begin{align}
    \label{eq:idk_nr_2}
    u(x) = u()
\end{align}



\appendix

\section{Deriving first derivative for $u$, from taylor expansion of $u(x)$ around $x=x+h$}




\begin{align*}
   eh 
\end{align*}
\end{document}